Strata/DL/Util/List.lean
@@ -415,4 +415,10 @@ theorem foldlM_empty {α β} {m:Type → Type} [Monad m]:
   ∀ (init:β) (f:β → α → m β),
     List.foldlM f init [] = Pure.pure init := by grind
 
+theorem all_forall_mem:
+  ∀ {T} (l:List T) P, l.all P = true ↔ (∀ m, m ∈ l → P m) := by grind
+
+theorem any_exists:
+  ∀ {T} (l:List T) P, l.any P = true ↔ (∃ m, m ∈ l ∧ P m) := by grind
+
 end List
